$$
\newcommand{\d}{\mathrm{d}}
$$

# 1.5 Linear ODE

#### Practice Problems 4

##### 1. 

$$
\dot x = cr - \cfrac{r}{V}·x
$$

Units Check: the unit of LHS $\d s/\d t$ is $\mathrm{g·min^{-1}}$, which represents the increase speed of the amount of salt, and the unit of $cr$ is $\mathrm{g·L^{-1}·{L·min^{-1}}=g·min^{-1}}$, and the unit of rx/V is $\mathrm{L·min^{-1}/L·g = g·min^{-1}}$. This conclues that the units of this ODE is right.

Convert it into an standard form:
$$
\dot x + \cfrac{r}{V}x = cr
$$
where the $p(x)$ is $r/V$ and the $q(x)$ is $cr$.



##### 2.

According the given assumptions, we got the ODE
$$
\dot x + 2x = 2c
$$
We've known the solution like that kind of equations in the superposition principle toturial, and we've known that the **general solution** of equation $\dot x +2x = 1$ is $x(t) = 1/2 + Ce^{-2t}$, with superposition principle appiled, we now that the general solution of our equation must be
$$
x(t) = c + Ce^{-2t}
$$
**P.S.** With the integrating factors technic applied, we can sovle it directly too, practically, since $\int 2 = 2t$ so the integral factor is $e^{2t}$, so we multiply it in both sides:
$$
\dot x · e^{2t} + 2xe^{2t} = 2ce^{2t}
$$
Then the LHS can be rewrite as a single derivative:
$$
(xe^{2t})' = 2ce^{2t}
$$
Integrate at both sides, then we got
$$
xe^{2t} = ce^{2t} + C
$$
as the result 
$$
x = c + Ce^{-2t}
$$
It's the same with the privious result, so the superposition method passed the test!



And with the IC $x(0) = 0$ applied, we got $ 0 = c + C$, so $C = -c$,
$$
x = c - ce^{-2t} = c(1-e^{-2t})
$$
It's a increasing function, as the time going to infinite,
$$
\lim_{t\rightarrow+\infin} c(1-e^{-2t}) = c
$$
so the limited amount of the tank is $c$. It's logic beacuse the $V=1 L$ so this represtents the concentration inside the bank is the same as the concentration of the added flow.

When $x = 1/2c$,
$$
c(1-e^{-2t}) = 1/2c
$$
the root is $t = \cfrac{\ln2}{2}$.



##### 3. 

It's similar with the previous condition but the $c$ is no longer a constant but a dependent variable $c(t)$, changing along the time is changed, based on the result we got at Problem 2, where we got that $x(t) = c(1-e^{-2t})$, and because the volumn is 1, so $c(t) = x(t)$. 

the ODE of the second tank is expressed as
$$
\dot x + 2x = 2c(1-e^{-2t})
$$
This is already the standard linear form. Still, we try to use the superposition method and the integrating factor method to solve this, we've know the solution of these two following ODE: 
$$
\dot x + 2x = 2c \rightarrow x = c + Ce^{-2t} \\
\dot x + 2x = e^{-2t} \rightarrow x = te^{-2t} + Ce^{-2t}
$$
With the old-fashion superposition principle appiled, the solution of our original equation must be
$$
x = c - 2cte^{-2t} + Ce^{-2t}
$$
With the direct way, still, we multiply $e^{2t}$ in both sides (because the $p(t) = 2$ has not changed), 
$$
\begin{align}
\dot xe^{2t} + 2xe^{2t} &= 2ce^{2t} - 2c 	\\
(xe^{2t})' &= 2ce^{2t} - 2c 					\\
xe^{2t} &= ce^{2t} - 2ct + C					\\
x &= c - 2cte^{-2t} + Ce^{-2t}				\\
\end{align}
$$

It the same with the previous result!



##### 4.

Since $V$ is a constant, $\d V/\d t \equiv 0$, the ODE is homogeneous.
$$
R\cfrac{\d I}{\d t} + \cfrac{1}{C}I = 0
$$
Separate the variables,
$$
\cfrac{\d I}{I} = -\cfrac{1}{RC}\d t \\
\ln|I| = -t/RC + c \\
I = ce^{-\frac{t}{RC}}
$$

with initial condition $I(0) = I_0$, we got $c = I_0$, so
$$
I = I_0e^{-\frac{t}{RC}}
$$
and $\tau = RC$.
$$
I(t+\tau) = \cfrac{I_0e^{-t/RC}}{e} = \cfrac{I(t)}{e}
$$
Which gives out that the current decrease to $1/e$ of the last time every $RC$ time passed.