# Radical Expressions Simplification

Example. The general method to simpliy the radical expression is **completing the square**, same as solving the quadratic equation.

Examples.

> $\sqrt{4+2\sqrt3} = \sqrt{\sqrt3^2 + 2\sqrt3 + 1} = \sqrt3 + 1$

> $\sqrt{2-\sqrt3} = \dfrac{\sqrt{2}}{2}\sqrt{4-2\sqrt3} = \dfrac{\sqrt{2}}{2}(\sqrt3 - 1) = \dfrac{\sqrt6-\sqrt2}{2}$

> $\sqrt{2a^2-b^2+2a\sqrt{a^2-b^2}} = \sqrt{a^2-b^2+2a\sqrt{a^2-b^2}+a^2} = \sqrt{\left(a - \sqrt{a^2-b^2}\right)^2}$
>
> Notice that $a > \sqrt{a^2-b^2}$, hence we have
> $$
> \sqrt{\left(a - \sqrt{a^2-b^2}\right)^2}
> = \left| a - \sqrt{a^2-b^2} \right|
> = a - \sqrt{a^2-b^2}
> $$

Generally, if the expression inside the equation is the form $a\pm 2\sqrt b = (\sqrt x+ \sqrt y)^2$, we can solve the equation by coefficient comparison. This can be applied if the factor is hard to see. For example, for the example $\sqrt{4+2\sqrt 3}$, Let $4 + 2\sqrt3 = x + y + 2\sqrt{xy}$, we solve the equation
$$
\left\{\begin{array}{ll}
x + y = 4 \\
xy = 3
\end{array}\right.

\Rightarrow

\left\{\begin{array}{ll}
x = 3 \\
y =1
\end{array}\right.
$$




